theories/Ref/SpecMFacts.v
@@ -1,0 +1,182 @@
+From Coq Require Export
+     Morphisms
+     Setoid
+     Program.Equality
+     Lists.List
+     Logic.EqdepFacts
+     Eqdep EqdepFacts
+.
+
+From EnTree Require Import
+     Basics.HeterogeneousRelations
+     Basics.QuantType
+     Core.EnTreeDefinition
+     Core.SubEvent
+     Ref.EnTreeSpecDefinition
+     Ref.EnTreeSpecFacts
+     Ref.EnTreeSpecCombinatorFacts
+     Ref.SpecM
+     Eq.Eqit
+     Ref.MRecSpec
+.
+
+Import SpecMNotations.
+Local Open Scope entree_scope.
+
+From Paco Require Import paco.
+
+Section interp_mrec_spec_quantl.
+Context (D E F: Type) `{EncodingType D} `{EncodingType E} `{EncodingType F}.
+Context (body : forall d : D, entree_spec (D + E) (encodes d)).
+Context (RPre : Rel E F ) (RPost : PostRel E F).
+Context (R1 R2 : Type) (RR : Rel R1 R2).
+
+Lemma interp_mrec_spec_forall A `{QuantType A} : 
+  interp_mrec_spec body (forall_spec A) ≅ forall_spec A.
+Proof.
+  pstep. red. cbn. constructor. intros. left. pstep. constructor.
+  auto.
+Qed.
+
+Lemma interp_mrec_spec_exists A `{QuantType A} : 
+  interp_mrec_spec body (exists_spec A) ≅ exists_spec A.
+Proof.
+  pstep. red. cbn. constructor. intros. left. pstep. constructor.
+  auto.
+Qed.
+
+Lemma interp_mrec_spec_assume P : 
+  interp_mrec_spec body (assume_spec P) ≅ assume_spec P.
+Proof.
+  pstep. red. cbn. constructor. intros. left. pstep. constructor.
+  auto.
+Qed.
+
+Lemma interp_mrec_spec_assert P : 
+  interp_mrec_spec body (assert_spec P) ≅ assert_spec P.
+Proof.
+  pstep. red. cbn. constructor. intros. left. pstep. constructor.
+  auto.
+Qed.
+
+Lemma padded_refines_assumel (P : Prop) (HP : P) k phi:
+  padded_refines RPre RPost RR (k tt) phi ->
+  padded_refines RPre RPost RR (EnTree.bind (assume_spec P) k) phi.
+Proof.
+  intros. setoid_rewrite bind_bind. apply padded_refines_forall_specl.
+  eauto.
+Qed.
+
+Lemma padded_refines_assertl (P : Prop)  k phi:
+  (P -> padded_refines RPre RPost RR (k tt) phi) ->
+  padded_refines RPre RPost RR (EnTree.bind (assert_spec P) k) phi.
+Proof.
+  intros. setoid_rewrite bind_bind. apply padded_refines_exists_specl.
+  eauto.
+Qed.
+
+Lemma interp_mrec_spec_forall_specl (A : Type) `{QuantType A} k phi (a : A) : 
+  padded_refines RPre RPost RR (interp_mrec_spec body (k a)) phi ->
+  padded_refines RPre RPost RR (interp_mrec_spec body (EnTree.bind (forall_spec A) k )) phi.
+Proof.
+  intros. setoid_rewrite interp_mrec_spec_bind.
+  rewrite interp_mrec_spec_forall. apply padded_refines_forall_specl.
+  eauto.
+Qed.
+
+Lemma interp_mrec_spec_exists_specl (A : Type) `{QuantType A} k phi : 
+  (forall (a : A), padded_refines RPre RPost RR (interp_mrec_spec body (k a)) phi) ->
+  padded_refines RPre RPost RR (interp_mrec_spec body (EnTree.bind (exists_spec A) k )) phi.
+Proof.
+  intros. setoid_rewrite interp_mrec_spec_bind.
+  rewrite interp_mrec_spec_exists. apply padded_refines_exists_specl.
+  eauto.
+Qed.
+
+Lemma interp_mrec_spec_assumel (P : Prop) (HP : P) k phi:
+  padded_refines RPre RPost RR (interp_mrec_spec body (k tt)) phi ->
+  padded_refines RPre RPost RR (interp_mrec_spec body (EnTree.bind (assume_spec P) k) ) phi.
+Proof.
+  intros. rewrite interp_mrec_spec_bind.
+  rewrite interp_mrec_spec_assume.
+  setoid_rewrite bind_bind. apply padded_refines_forall_specl.
+  exists HP. rewrite bind_ret_l. auto.
+Qed.
+
+Lemma interp_mrec_spec_assertl (P : Prop) k phi : 
+  (P -> padded_refines RPre RPost RR (interp_mrec_spec body (k tt)) phi) -> 
+  padded_refines RPre RPost RR (interp_mrec_spec body (EnTree.bind (assert_spec P) k) ) phi.
+Proof.
+  intros. rewrite interp_mrec_spec_bind.
+  rewrite interp_mrec_spec_assert. setoid_rewrite bind_bind.
+  apply padded_refines_exists_specl. auto.
+Qed.
+
+
+
+End interp_mrec_spec_quantl.
+
+Section interp_mrec_spec_quantr.
+
+Context (D E F: Type) `{EncodingType D} `{EncodingType E} `{EncodingType F}.
+Context (body : forall d : D, entree_spec (D + F) (encodes d)).
+Context (RPre : Rel E F ) (RPost : PostRel E F).
+Context (R1 R2 : Type) (RR : Rel R1 R2).
+
+
+Lemma interp_mrec_spec_forall_specr (A : Type) `{QuantType A} k phi : 
+  (forall (a : A), padded_refines RPre RPost RR phi (interp_mrec_spec body (k a))) ->
+  padded_refines RPre RPost RR phi (interp_mrec_spec body (EnTree.bind (forall_spec A) k )).
+Proof.
+  intros. setoid_rewrite interp_mrec_spec_bind.
+  rewrite interp_mrec_spec_forall. apply padded_refines_forall_specr.
+  eauto.
+Qed.
+
+Lemma interp_mrec_spec_exists_specr (A : Type) `{QuantType A} k phi (a : A) : 
+  (padded_refines RPre RPost RR phi (interp_mrec_spec body (k a))) ->
+  padded_refines RPre RPost RR phi (interp_mrec_spec body (EnTree.bind (exists_spec A) k )).
+Proof.
+  intros. setoid_rewrite interp_mrec_spec_bind.
+  rewrite interp_mrec_spec_exists. apply padded_refines_exists_specr.
+  eauto.
+Qed.
+
+Lemma padded_refines_assumer (P : Prop) k phi :
+  (P -> padded_refines RPre RPost RR phi (k tt)) ->
+  padded_refines RPre RPost RR phi ((EnTree.bind (assume_spec P) k)).
+Proof.
+  intros. setoid_rewrite bind_bind.
+  apply padded_refines_forall_specr. auto.
+Qed.
+
+Lemma padded_refines_assertr (P : Prop) (HP : P) k phi :
+  padded_refines RPre RPost RR phi (k tt) ->
+  padded_refines RPre RPost RR phi ((EnTree.bind (assert_spec P) k)).
+Proof.
+  intros. setoid_rewrite bind_bind.
+  apply padded_refines_exists_specr. eauto.
+Qed.
+
+Lemma interp_mrec_spec_assumer (P : Prop) k phi :
+  (P -> padded_refines RPre RPost RR phi (interp_mrec_spec body (k tt))) ->
+  padded_refines RPre RPost RR phi (interp_mrec_spec body (EnTree.bind (assume_spec P) k)).
+Proof.
+  intros. rewrite interp_mrec_spec_bind.
+  rewrite interp_mrec_spec_assume.
+  setoid_rewrite bind_bind.
+  apply padded_refines_forall_specr. auto.
+Qed.
+
+Lemma interp_mrec_spec_assertr (P : Prop) (HP : P) k phi :
+  padded_refines RPre RPost RR phi (interp_mrec_spec body (k tt)) ->
+  padded_refines RPre RPost RR phi (interp_mrec_spec body (EnTree.bind (assert_spec P) k)).
+Proof.
+  intros. rewrite interp_mrec_spec_bind.
+  rewrite interp_mrec_spec_assert.
+  setoid_rewrite bind_bind.
+  apply padded_refines_exists_specr. exists HP.
+  auto.
+Qed.
+
+End interp_mrec_spec_quantr.
